New language. Other difficulties to make WP work.

theories/heap_lang/lang.v
@@ -11,7 +11,7 @@ Parameter state : Type.
 Parameter action : Type.
 Parameter condition : Type.
 
-Parameter apply_action : state -> action -> state.
+Parameter apply_action : state -> action -> state -> Prop.
 
 Parameter action_eq : EqDecision action.
 Declare Instance : EqDecision action.
@@ -25,6 +25,10 @@ Declare Instance : Countable condition.
 
 Parameter CTrue : condition.
 Parameter CFalse : condition.
+
+Parameter DCTrueCFalse : CTrue <> CFalse.
+
+Parameter condition_reduce : condition -> state -> condition -> Prop.
 
 Module heap_lang.
 Open Scope Z_scope.
@@ -43,28 +47,12 @@ Inductive command :=
   positions.
   However, some commands need to be reduced in several steps.
   For instance, an [Assert C] command must first reduce to a
-  [Assert CTrue] command to be executed.
-  I also added an [Error] case.  This is not a return value:
-  it is just an expression with no semantics.  It is being
-  needed as Iris supposes that the [fill_item] function is
-  total, which is obviously not the case in a typed setting.
-  I thus need a dummy expression for this case.  A better
-  fix would be to change Iris altogether to make it accept
-  non-total [fill_item] functions. **)
-
-(** Expect that this would not ork because Iris forces the
-  [fill_item] function to take an expression (Iris has
-  clearly not be done with types in mind… at least not in
-  the analysed programming laguage—this is so frustrating!)
-  and not something else, like a condition.  We could add
-  again a dummy case for that, but this is going to be too
-  strange. **)
+  [Assert CTrue] command to be executed. **)
 
 Inductive expression :=
   | PC (pc : position)
   | PCC (pc : position) (c : command)
   | Halted
-  | Error
   .
 
 Definition program := list command.
@@ -128,23 +116,21 @@ Definition encode_expression e :=
   match e with
   | PC pc => inl (inl pc)
   | PCC pc c => inl (inr (pc, c))
-  | Halted => inr (inl ())
-  | Error => inr (inr ())
+  | Halted => inr ()
   end.
 
 Definition decode_expression e :=
   match e with
   | inl (inl pc) => PC pc
   | inl (inr (pc, c)) => PCC pc c
-  | inr (inl ()) => Halted
-  | inr (inr ()) => Error
+  | inr () => Halted
   end.
 
 Instance expression_countable : Countable expression.
 Proof. refine (inj_countable' encode_expression decode_expression _); by intros []. Qed.
 
 Instance command_inhabited : Inhabited command := populate (Assert CFalse).
-Instance expression_inhabited : Inhabited expression := populate Error.
+Instance expression_inhabited : Inhabited expression := populate Halted.
 
 Canonical Structure ssstateC := leibnizC ssstate.
 Canonical Structure commandC := leibnizC command.
@@ -153,65 +139,61 @@ Canonical Structure expressionC := leibnizC expression.
 
 (** Evaluation contexts **)
 
-(** The only cases when we use evaluation contexts in this language is when a condition
-   has to be reduced to either [CTrue] or [CFalse].  This can happen in either the
-   [JumpIf] case or the [Assert] case. **)
+(** The only cases whee we could use evaluation contexts in this language
+   is when a condition  has to be reduced to either [CTrue] or [CFalse].
+   This can happen in either the [JumpIf] case or the [Assert] case.
+   However, the type constraints on the function [fill_context] in Iris
+   assume that (1) the function [fill_context] is from expressions to
+   expressions, and (2), that it is complete.  The first issue is
+   problematical as in the only place where contexts appear in our
+   language, contexts take conditions and not expressions.  In other
+   words, our language is sorted: conditions are not commands.  We could
+   solve this issue by stating that expressions consider all possible
+   sorts of our language, but then the issue (2) comes into place: what
+   is the result of filling a context with an object of a different
+   type than its hole?  This is of course meaningless.  Iris’s contexts
+   are thus not suitable for our language.  This is frustrating, given
+   the simplicity of our example. **)
 
-Inductive context :=
-  | context_JumpIf (pc : position) (target : position)
-
-Definition command_eval (st : state) (pc : position) (c : command) : option (state * position) :=
-  match c with
-  | Action a => Some (apply_action st a, Pos.add 1 pc)
-  | JumpIf target C =>
-    if test_condition st C then Some (st, target)
-    else None
-  | Assert C =>
-    if test_condition st C then Some (st, Pos.add 1 pc)
-    else None
-  end.
-
-Definition position_eval (st : state) (p : program) (pc : position) : option (state * option position) :=
-  match read p pc with
-  | None => Some (st, None)
-  | Some c =>
-    match command_eval st pc c with
-    | None => None
-    | Some (st, p) => Some (st, Some p)
-    end
-  end.
-
-(** In this language, what is called the state in Iris includes the program. **)
-Definition full_state : Type := state * program.
-
-Inductive head_step : option position → full_state → option position → full_state → list (option position) → Prop :=
-  | head_step_cons pc st p st' pc' :
-    position_eval st p pc = Some (st', pc') ->
-    head_step (Some pc) (st, p) pc' (st', p) []
-  .
-
-(** There is only one value: the [None] construct, where the program is halted **)
-Definition value := unit.
-
-Definition of_value (_ : unit) : option position := None.
-Definition to_value (pc : option position) :=
-  match pc with
-  | None => Some tt
-  | Some _ => None
-  end.
-
-(** Similarly, evaluation contexts are useless in such a language. **)
 Definition context : Type := False.
 
-Definition fill_context (K : context) : option position -> option position :=
+Definition fill_context (K : context) : expression -> expression :=
   match K with end.
 
-Lemma heap_lang_mixin : EctxiLanguageMixin of_value to_value fill_context head_step.
+Inductive head_step : expression -> ssstate -> expression -> ssstate -> list expression -> Prop :=
+  | head_step_halt p st pc :
+    read p pc = None ->
+    head_step (PC pc) (st, p) Halted (st, p) []
+  | head_step_read p st pc c :
+    read p pc = Some c ->
+    head_step (PC pc) (st, p) (PCC pc c) (st, p) []
+  | head_step_action p st st' pc a :
+    apply_action st a st' ->
+    head_step (PCC pc (Action a)) (st, p) (PC (1 + pc)%positive) (st', p) []
+  | head_step_jump_reduce p st pc target C C' :
+    condition_reduce C st C' ->
+    head_step (PCC pc (JumpIf target C)) (st, p) (PCC pc (JumpIf target C')) (st, p) []
+  | head_step_assert_reduce p st pc C C' :
+    condition_reduce C st C' ->
+    head_step (PCC pc (Assert C)) (st, p) (PCC pc (Assert C')) (st, p) []
+  | head_step_jump_true p st pc target :
+    head_step (PCC pc (JumpIf target CTrue)) (st, p) (PC target) (st, p) []
+  | head_step_jump_false p st pc target :
+    head_step (PCC pc (JumpIf target CFalse)) (st, p) (PC (1 + pc)%positive) (st, p) []
+  | head_step_assert_true p st pc :
+    head_step (PCC pc (Assert CTrue)) (st, p) (PC (1 + pc)%positive) (st, p) []
+  .
+
+Lemma heap_lang_mixin : EctxiLanguageMixin of_val to_val fill_context head_step.
 Proof.
   split; repeat intro; repeat match goal with v : unit |- _ => destruct v end; auto;
-    try solve [ repeat match goal with pc : option _ |- _ => destruct pc
+    try solve [ repeat match goal with
+                | e : expression |- _ => destruct e
                 | H : _ |- _ => solve [ inversion H ] end; auto ].
 Qed.
+
+Lemma val_stuck e1 σ1 e2 σ2 efs : head_step e1 σ1 e2 σ2 efs → to_val e1 = None.
+Proof. destruct 1; naive_solver. Qed.
 
 End heap_lang.
 
